coxeter move as inductive type

DemazureOperators/Matsumoto.lean
@@ -1,41 +1,53 @@
 import DemazureOperators.Coxeter
-
-variable {B : Type*} [DecidableEq B]
-
-structure Move where
-  pre : List B
-  post : List B
-
-def apply_move (s : Move) (l : List B) :=
-  if l.take s.pre.length = s.pre then
-    s.post ++ l.drop s.pre.length
-  else
-    l
-
-#eval apply_move {pre := [1, 2], post := [3, 4]} [1, 2, 3, 4, 5]
-
-def nil_move (i : B) : @Move B := {pre := [i, i], post := []}
-
 open CoxeterSystem
 
 variable {B : Type}  [DecidableEq B]
 variable {W : Type} [Group W] [DecidableEq W]
 variable {M : CoxeterMatrix B} (cs : CoxeterSystem M W)
 
+inductive CoxeterMove (cs : CoxeterSystem M W) where
+| nil (i : B) : CoxeterMove cs
+| braid (i j : B) : CoxeterMove cs
+
+def apply_coxeterMove (s : CoxeterMove cs) (l : List B) : List B :=
+  match s with
+  | CoxeterMove.nil i =>
+    if l.take 2 = [i, i] then
+      l.drop 2
+    else
+      l
+  | CoxeterMove.braid i j =>
+    if l.take (M i j) = braidWord M i j then
+      braidWord M i j ++ l.drop (M i j)
+    else
+      l
+
 local prefix:100 "s" => cs.simple
 local prefix:100 "π" => cs.wordProd
 local prefix:100 "ℓ" => cs.length
 
-theorem nil_move_wordProd (i : B) (l : List B) : π (apply_move (nil_move i) l) = π l := by
-  simp [apply_move, nil_move]
-  by_cases h: l.take 2 = [i, i]
-  · simp[h]
-    have h' : l = l.take 2 ++ l.drop 2 := by simp
-    nth_rewrite 2 [h']
-    rw[wordProd_append]
-    rw[h]
+theorem coxeterMove_wordProd (cm : CoxeterMove cs) (l : List B) : π (apply_coxeterMove cs cm l) = π l := by
+  simp [apply_coxeterMove]
+  cases cm with
+  | nil i =>
     simp
-    convert_to cs.wordProd ([i] ++ [i]) = 1
-    rw[wordProd_append]
+    by_cases h : l.take 2 = [i, i]
+    · simp[h]
+      have h' : l = l.take 2 ++ l.drop 2 := by simp
+      nth_rewrite 2 [h']
+      rw[wordProd_append]
+      rw[h]
+      simp
+      convert_to cs.wordProd ([i] ++ [i]) = 1
+      rw[wordProd_append]
+      simp
+    · simp[h]
+  | braid i j =>
     simp
-  · simp[h]
+    by_cases h : List.take (M.M i j) l = braidWord M i j
+    · simp[h]
+      have h' : l = l.take (M.M i j) ++ l.drop (M.M i j) := by simp
+      nth_rewrite 2 [h']
+      repeat rw[wordProd_append]
+      rw[h]
+    · simp[h]
